Debug (#132)
This PR fixes several bugs - mostly involving mismatches in “serialized”
types. To make debugging easier, it changes the signature of the
resource-logic function: it is now monadic, maintains a stack trace, and
returns a descriptive error instead of simply `false` on failure.

I also fixed the monadic version of the `check` macro, which was not
working correctly. I had to rename it to `docheck` to avoid conflicts
with the term-level `check`.

Finally, I added a rather hacky mechanism, `mydefaultM`, to report the
location of logic-function errors even when there is no explicit
`failwith` clause. We should keep this for now but plan to remove it
later.

I've also added a tiny example - a program with a single constructor
call - that runs on CI.

Anoma/Logic.lean
@@ -2,6 +2,27 @@ import Anoma.Resource
 
 namespace Anoma
 
+structure LogicM.Error : Type where
+  stackTrace : List String
+  position : FilePosition
+  reason : String
+
+def LogicM.Error.onlyPosition (position : FilePosition) : LogicM.Error where
+  position
+  stackTrace := []
+  reason := "<no explicit reason>"
+
+def LogicM.Error.custom (position : FilePosition) (reason : String) : LogicM.Error where
+  position
+  stackTrace := []
+  reason
+
+instance : Repr LogicM.Error where
+  reprPrec e _ :=
+    s!"Error at {repr e.position}
+      Reason:\n{e.reason}
+      Trace:\n{e.stackTrace.unlines}"
+
 structure Logic.Args : Type 2 where
   self : Resource
   status : ConsumedCreated
@@ -11,9 +32,37 @@ structure Logic.Args : Type 2 where
   Data : SomeType.{0}
   data : Data.type
 
+-- The StackTrace is only used in the error message. It should never be used to
+-- branch on a computation.
+abbrev LogicM.StackTrace := List String
+
 def Logic.Args.isConsumed (d : Logic.Args) := d.status.isConsumed
 
-abbrev LogicFunction : Type 2 := Logic.Args → Bool
+abbrev LogicM : Type := EStateM LogicM.Error LogicM.StackTrace Unit
+
+abbrev LogicM.true : LogicM := pure .unit
+
+abbrev LogicM.eval (l : LogicM) : Option LogicM.Error :=
+  match l.run ∅ with
+  | .error e _ => some e
+  | .ok _ _ => none
+
+abbrev LogicM.withTrace (here : FilePosition) (str : String) (l : LogicM) : LogicM := do
+  let old ← get
+  set (s!"{repr here}: {str}" :: old)
+  l
+  set old
+
+abbrev LogicM.isOk (l : LogicM) : Bool := l.eval.isNone
+
+def LogicM.throw (position : FilePosition) (reason : String) : LogicM := do
+  let s ← get
+  MonadExcept.throw
+    { reason
+      position
+      stackTrace := s.reverse }
+
+def LogicFunction : Type 2 := Logic.Args → LogicM
 
 structure Logic where
   reference : LogicRef
