AVM/Label.lean
@@ -11,10 +11,19 @@ structure Object.Resource.Label where
   /-- The dynamic label is used to put dynamic data into the Resource label -/
   dynamicLabel : classId.label.DynamicLabel.Label.type
 
+instance : Repr Object.Resource.Label where
+  reprPrec l _ :=
+    have := l.label.classesRepr
+    s!"Resource.Label@\{
+      label := {repr l.label}
+      classId := {repr l.classId}
+      dynamicLabel := ?
+   }"
+
 instance : Hashable Object.Resource.Label where
   hash l := Hashable.Mix.run do
     mix l.label
-    mix (l.label.classesEnum.equiv l.classId)
+    mix l.classId.nat
     have := l.classId.label.DynamicLabel.Label.typeHashable
     mix l.dynamicLabel
 
@@ -39,6 +48,11 @@ instance : Hashable Resource.Label where
     | .message s =>
       mix 1
       mix s
+
+instance : Repr Resource.Label where
+  reprPrec lab _prec := match lab with
+    | .object l => s!"object:{repr l}"
+    | .message l => s!"message:{repr l}"
 
 instance : TypeRep Resource.Label where
   rep := Rep.atomic "AVM.Resource.Label"
