AVM/Message/Base.lean
@@ -9,6 +9,9 @@ structure Message (lab : Ecosystem.Label) : Type 1 where
   /-- Signatures for `data`. -/
   signatures : List Signature
 
+instance {lab : Ecosystem.Label} : Repr (Message lab) where
+  reprPrec r _ := repr r.data
+
 def Message.rawSignatures {lab : Ecosystem.Label} (msg : Message lab) : List Nat :=
   msg.signatures.map Signature.raw
 
@@ -26,6 +29,9 @@ instance Message.hasBEq {lab : Ecosystem.Label} : BEq (Message lab) where
 structure SomeMessage : Type 1 where
   {label : Ecosystem.Label}
   message : Message label
+
+instance SomeMessage.instRepr : Repr SomeMessage where
+  reprPrec m _ := repr m.message
 
 instance SomeMessage.instHashable : Hashable SomeMessage where
   hash m := Hashable.Mix.run do
