AVM/Program/Parameters.lean
@@ -39,6 +39,9 @@ def Product (params : Program.Parameters) : Type :=
   | .rand rest =>
     Σ (r : Nat), Program.Parameters.Product (rest r)
 
+instance Product.instRepr {params : Program.Parameters} : Repr (Product params) where
+  reprPrec _ _ := "Product {..}"
+
 def Product.hashHelper {params : Program.Parameters} (p : params.Product) : Hashable.Mix := do
   match params with
   | .empty =>
