Applib/Surface/Program/Syntax.lean
@@ -16,12 +16,12 @@ def elabClosedNat (t : Syntax) : TacticM Nat := do
     reduceEval e
 
 def findProof (scope : Term) : TacticM Unit := do
-  let card <- elabClosedNat (← `(term| (AVM.Scope.Label.EcosystemIdEnum $scope).1))
+  let card <- elabClosedNat (← `(term| (AVM.Scope.Label.EcosystemIdEnum $scope).card))
   let f ← `(term| ($scope).EcosystemIdEnum.equiv.invFun)
   let possibleIndices : List (Fin card) := List.finRange card
   let tryN (n : Fin card) : TacticM Unit := do
     let sn := Syntax.mkNumLit (toString n)
-    let labelId ← `(term| $f $sn)
+    let labelId : TSyntax `term ← `(term| $f $sn)
     let t ← `(tactic| try exact ⟨$labelId, by rfl⟩)
     evalTactic t
   for x in possibleIndices do
