Prelude/Check.lean
@@ -1,22 +1,48 @@
-import Lean.Parser.Term
-
-open Lean.Parser.Term
+import Prelude.Macro
+import Prelude.CustomDefault
 
 syntax withPosition("check" term) optSemicolon(term)? : term
 syntax withPosition("check " binderIdent " : " term) optSemicolon(term) : term
 syntax withPosition("check" term) optSemicolon(doSeq) : doElem
 syntax withPosition("check " binderIdent " : " term) optSemicolon(doSeq) : doElem
 
+syntax withPosition("check" term) withPosition("failwith" term) optSemicolon(term)? : term
+syntax withPosition("check " binderIdent " : " term) withPosition("failwith" term) optSemicolon(term) : term
+syntax withPosition("check" term) withPosition("failwith" term) optSemicolon(doSeq) : doElem
+
+syntax withPosition("docheck " binderIdent " : " term) withPosition("failwith" term) optSemicolon(doSeq) : doElem
+syntax withPosition("docheck" term) optSemicolon(doSeq) : doElem
+syntax withPosition("docheck " binderIdent " : " term) optSemicolon(doSeq) : doElem
+syntax withPosition("docheck" term) withPosition("failwith" term) optSemicolon(doSeq) : doElem
+
+
 /-- The `check a; b` macro returns `b` if `a` evaluates to `true`, or `default`
   otherwise. -/
 macro_rules
 | `(check $cond:term ; $body:term) =>
-  `(if $cond then $body else default)
+  `(if $cond then $body else by mydefault)
 | `(check $h:ident : $cond:term ; $body:term) =>
-  `(if $h:ident : $cond then $body else default)
+  `(if $h:ident : $cond then $body else by mydefault)
 | `(check $cond:term) =>
   `($cond)
-| `(doElem| check $cond:term ; $body:doSeq) =>
-  `(doElem| if $cond then $body else pure default)
-| `(doElem| check $h:ident : $cond:term ; $body:doSeq) =>
-  `(doElem| if $h : $cond then $body else pure default)
+| `(doElem| docheck $cond:term ; $body:doSeq) =>
+  `(doElem| if $cond then $body else by mydefaultM)
+| `(doElem| docheck $h:ident : $cond:term ; $body:doSeq) =>
+  `(doElem| if $h : $cond then $body else by mydefaultM)
+
+| `(check $cond:term failwith $f:term ; $body:term) =>
+  `(if $cond then $body else $f)
+| `(check $h:ident : $cond:term failwith $f:term ; $body:term) =>
+  `(if $h:ident : $cond then $body else $f)
+| `(check $cond:term failwith $f) =>
+  `(if $cond then true else $f)
+| `(doElem| docheck $cond:term failwith $f:term ; $body:doSeq) => do
+  let errDo : TSyntax `Lean.Parser.Term.doSeq ← doSeq1 (← `(term| $f))
+  `(doElem| if $cond then $body else $errDo)
+| `(doElem| docheck $h:ident : $cond:term failwith $f:term ; $body:doSeq) => do
+  let errDo : TSyntax `Lean.Parser.Term.doSeq ← doSeq1 (← `(term| $f))
+  `(doElem| if $h : $cond then $body else $errDo)
+
+example [Monad m] : m Unit := do
+  docheck 0 == 0
+  pure .unit
