Prelude/CustomDefault.lean
@@ -1,0 +1,26 @@
+import Lean
+import Prelude.Debug
+
+open Lean
+open Elab.Tactic Meta
+
+elab "mydefault" : tactic => do
+   let tgt ← getMainTarget
+   if tgt.isAppOf `Anoma.LogicM
+     then
+        let rawErr : TSyntax `term := mkIdent `Anoma.LogicM.Error.onlyPosition
+        let t ← `(tactic| exact (throw ($rawErr here#)))
+        evalTactic t
+     else do
+      let t ← `(tactic| exact default)
+      evalTactic t
+
+elab "mydefaultM" : tactic => do
+   let tgt ← getMainTarget
+   if tgt.isAppOf `LogicM
+     then
+        let t ← `(tactic| exact (throw (LogicM.Error.onlyPosition here#)))
+        evalTactic t
+     else do
+      let t ← `(tactic| exact (pure default))
+      evalTactic t
