Prelude/Debug.lean
@@ -1,0 +1,27 @@
+import Lean
+
+open Lean
+
+structure FilePosition where
+  file : String
+  pos : Position
+  deriving ToExpr
+
+instance : Repr FilePosition where
+  reprPrec p _ := s!"{p.file}:{p.pos.line}:{p.pos.column}"
+
+def FilePosition.unknown : FilePosition where
+  file := "<unknown-file>"
+  pos := ⟨0, 0⟩
+
+-- returns FilePosition for the location where it is inserted
+elab "here#" : term => do
+  let file ← getFileName
+  let ref ← getRef
+  let fm ← getFileMap
+  let some pos := ref.getPos?
+    | return (toExpr FilePosition.unknown)
+  let lc : FilePosition :=
+         { file
+           pos := fm.toPosition pos }
+  return (toExpr lc)
