Prelude/LetTry.lean
@@ -1,9 +1,19 @@
+import Prelude.CustomDefault
+import Prelude.Macro
+
 syntax withPosition("let" "try" term (":" term)? ":=" term) optSemicolon(term) : term
 syntax withPosition("let" "try" term (":" term)? ":=" term) optSemicolon(doSeq) : doElem
 syntax withPosition("let" "try" term (":" term)? "←" term)  optSemicolon(doSeq) : doElem
 syntax withPosition("let" "try" term (":" term)? ":=" term) withPosition("failwith" term) optSemicolon(term) : term
 syntax withPosition("let" "try" term (":" term)? ":=" term) withPosition("failwith" doSeq) optSemicolon(doSeq) : doElem
 syntax withPosition("let" "try" term (":" term)? "←" term) withPosition("failwith" doSeq) optSemicolon(doSeq) : doElem
+
+syntax withPosition("let" "catch" term (":" term)? ":=" term) optSemicolon(term) : term
+syntax withPosition("let" "catch" term (":" term)? ":=" term) optSemicolon(doSeq) : doElem
+syntax withPosition("let" "catch" term (":" term)? "←" term)  optSemicolon(doSeq) : doElem
+syntax withPosition("let" "catch" term (":" term)? ":=" term) withPosition("failwith" term) optSemicolon(term) : term
+syntax withPosition("let" "catch" term (":" term)? ":=" term) withPosition("failwith" term) optSemicolon(doSeq) : doElem
+syntax withPosition("let" "catch" term (":" term)? "←" term) withPosition("failwith" doSeq) optSemicolon(doSeq) : doElem
 
 /-- The `let try x := ov; b` macro unwraps an `Option`, for `ov = some v` binds
   the value `v` to `x` in `b`, for `ov = none` returns `default`. The value
@@ -13,29 +23,49 @@ syntax withPosition("let" "try" term (":" term)? "←" term) withPosition("failw
   The type of `x` can be specified and `x` can be an arbitrary match pattern. -/
 macro_rules
 | `(let try $x:term := $e:term ; $body) =>
-  `(match ($e) with | none => default | some $x => $body)
+  `(match ($e) with | none => by mydefault | some $x => $body)
 | `(let try $x:term : $t:term := $e:term ; $body) =>
-  `(match ($e) with | none => default | some ($x : $t) => $body)
+  `(match ($e) with | none => by mydefault | some ($x : $t) => $body)
 | `(let try $x:term := $e:term failwith $r:term ; $body) =>
   `(match ($e) with | none => $r | some $x => $body)
 | `(let try $x:term : $t:term := $e:term failwith $r:term ; $body) =>
   `(match ($e) with | none => $r | some ($x : $t) => $body)
 | `(doElem| let try $x:term := $e:term ; $body) =>
-  `(doElem| match ($e) with | none => default | some $x => $body)
+  `(doElem| match ($e) with | none => by mydefaultM | some $x => $body)
 | `(doElem| let try $x:term : $t:term := $e:term ; $body) =>
-  `(doElem| match ($e) with | none => default | some ($x : $t) => $body)
+  `(doElem| match ($e) with | none => by mydefaultM | some ($x : $t) => $body)
 | `(doElem| let try $x:term := $e:term failwith $r:doSeq ; $body) =>
   `(doElem| match ($e) with | none => $r | some $x => $body)
 | `(doElem| let try $x:term : $t:term := $e:term failwith $r:doSeq ; $body) =>
   `(doElem| match ($e) with | none => $r | some ($x : $t) => $body)
 | `(doElem| let try $x:term ← $e:term ; $body) =>
-  `(doElem| match ← $e with | none => default | some $x => $body)
+  `(doElem| match ← $e with | none => by mydefaultM | some $x => $body)
 | `(doElem| let try $x:term : $t:term ← $e:term ; $body) =>
-  `(doElem| match ← $e with | none => default | some ($x : $t) => $body)
+  `(doElem| match ← $e with | none => by mydefaultM | some ($x : $t) => $body)
 | `(doElem| let try $x:term ← $e:term failwith $r:doSeq ; $body) =>
   `(doElem| match ← $e with | none => $r | some $x => $body)
 | `(doElem| let try $x:term : $t:term ← $e:term failwith $r:doSeq ; $body) =>
   `(doElem| match ← $e with | none => $r | some ($x : $t) => $body)
+
+| `(let catch $x:term := $e:term ; $body) =>
+  `(match ($e) with | .error err => .error err | .ok $x => $body)
+| `(let catch $x:term : $t:term := $e:term ; $body) =>
+  `(match ($e) with | .error err => .error err | .ok ($x : $t) => $body)
+| `(let catch $x:term := $e:term failwith $r:term ; $body) =>
+  `(match ($e) with | .error err => $r err | some $x => $body)
+| `(let catch $x:term : $t:term := $e:term failwith $r:term ; $body) =>
+  `(match ($e) with | .error err => $r err | .ok ($x : $t) => $body)
+
+| `(doElem| let catch $x:term := $e:term ; $body) =>
+  `(doElem| match ($e) with | Except.error err => .error err | .ok $x => $body)
+| `(doElem| let catch $x:term : $t:term := $e:term ; $body) =>
+  `(doElem| match ($e) with | Except.error err => Except.error err | .ok ($x : $t) => $body)
+| `(doElem| let catch $x:term := $e:term failwith $r:term ; $body) => do
+  let errSeq : TSyntax `Lean.Parser.Term.doSeq ← doSeq1 (← `(term| $r err))
+  `(doElem| match ($e) with | Except.error err => $errSeq | .ok $x => $body)
+| `(doElem| let catch $x:term : $t:term := $e:term failwith $r:term ; $body) => do
+  let errSeq : TSyntax `Lean.Parser.Term.doSeq ← doSeq1 (← `(term| $r err))
+  `(doElem| match ($e) with | Except.error err => $errSeq | .ok ($x : $t) => $body)
 
 /-
 #eval let try x := some 42; some (x + 1)
@@ -46,3 +76,8 @@ macro_rules
 #eval let try _ : Nat := none; true
 #eval let try (_, y) := some (1, 2); some (y + 1)
 -/
+
+example : Except String Unit := do
+  let catch _num : Nat := throw "test"
+    failwith fun (err : String) => throw err
+  pure .unit
