Prelude/Macro.lean
@@ -1,0 +1,13 @@
+import Lean.Parser.Do
+import Lean.Parser.Term
+
+open Lean
+open Parser
+open Term
+
+/-- Turn a `term` into a single-element `doSeq`. -/
+def doSeq1 (t : TSyntax `term) : MacroM (TSyntax ``doSeq) :=
+  `(doSeq| $t:term)
+
+export Lean (TSyntax)
+export Term (binderIdent)
